Libraries for hybrid language have proper names

Hybrid/EmptyEquivLib.v
@@ -7,46 +7,45 @@ Require Import Relations.
 
 Open Scope permut_scope.
 
-(* emptyEquiv = map (fun x => (x, nil)) (map fst G) *)
-Fixpoint emptyEquiv (G: Background_LF) : Background_LF :=
+(* emptyEquiv_Hyb = map (fun x => (x, nil)) (map fst G) *)
+Fixpoint emptyEquiv_Hyb (G: bg_Hyb) : bg_Hyb :=
 match G with
 | nil => nil
-| (w, a)::G => (w, nil) :: emptyEquiv G
+| (w, a)::G => (w, nil) :: emptyEquiv_Hyb G
 end.
 
-Add Morphism emptyEquiv : Permut_emptyEquiv.
+Add Morphism emptyEquiv_Hyb : Permut_emptyEquiv_Hyb.
 intros.
 induction H; simpl in *; auto.
-transitivity (emptyEquiv G'); auto.
+transitivity (emptyEquiv_Hyb G'); auto.
 Qed.
 
-
-Lemma emptyEquiv_last_change:
+Lemma emptyEquiv_Hyb_last_change:
 forall G G' w C C',
   G  ~=~ G'& (w, C) ->
-  emptyEquiv G ~=~ emptyEquiv (G' & (w, C')).
+  emptyEquiv_Hyb G ~=~ emptyEquiv_Hyb (G' & (w, C')).
 intros.
-assert (G ~=~ (w, C) :: G') by (transitivity (G' & (w,C)); PPermut_simpl).
-assert (G' & (w, C') ~=~ (w, C') :: G') by PPermut_simpl.
+assert (G ~=~ (w, C) :: G') by (transitivity (G' & (w,C)); PPermut_Hyb_simpl).
+assert (G' & (w, C') ~=~ (w, C') :: G') by PPermut_Hyb_simpl.
 rewrite H0; rewrite H1; simpl; auto.
 Qed.
 
-Lemma emptyEquiv_rewrite:
+Lemma emptyEquiv_Hyb_rewrite:
 forall G H,
-  emptyEquiv (G++H) = emptyEquiv G ++ emptyEquiv H.
+  emptyEquiv_Hyb (G++H) = emptyEquiv_Hyb G ++ emptyEquiv_Hyb H.
 induction G; rew_app; intros; auto.
 rew_app; destruct a; simpl; rew_app; rewrite IHG; auto.
 Qed.
 
-Lemma emptyEquiv_rewrite_last:
+Lemma emptyEquiv_Hyb_rewrite_last:
 forall G C,
-  emptyEquiv (G & C) = emptyEquiv G ++ emptyEquiv (C::nil).
-intros; apply emptyEquiv_rewrite.
+  emptyEquiv_Hyb (G & C) = emptyEquiv_Hyb G ++ emptyEquiv_Hyb (C::nil).
+intros; apply emptyEquiv_Hyb_rewrite.
 Qed.
 
-Lemma emptyEquiv_Mem_nil:
+Lemma emptyEquiv_Hyb_Mem_nil:
 forall G w C,
-  Mem (w, C) (emptyEquiv G) -> C = nil.
+  Mem (w, C) (emptyEquiv_Hyb G) -> C = nil.
 induction G; simpl; intros.
 rewrite Mem_nil_eq in H; contradiction.
 destruct a; simpl in *; rewrite Mem_cons_eq in H; destruct H.
@@ -54,111 +53,112 @@ inversion H; subst; auto.
 apply IHG with (w:=w); auto.
 Qed.
 
-Lemma emptyEquiv_permut_empty:
+Lemma emptyEquiv_Hyb_permut_empty:
 forall G G' w,
-  G ~=~ emptyEquiv G' ->
+  G ~=~ emptyEquiv_Hyb G' ->
   forall C, Mem (w, C) G -> C = nil.
 intros;
-assert (G ~=~ emptyEquiv G') by auto;
-apply PPermut_Mem with (w:=w) (X:=C) in H; auto;
+assert (G ~=~ emptyEquiv_Hyb G') by auto;
+apply PPermut_Hyb_Mem with (w:=w) (X:=C) in H; auto;
 destruct H as (C', (Ha, Hb)).
-apply emptyEquiv_Mem_nil in Hb; subst.
+apply emptyEquiv_Hyb_Mem_nil in Hb; subst.
 apply permut_nil_eq in Ha; auto.
 Qed.
 
-Lemma double_emptyEquiv:
+Lemma double_emptyEquiv_Hyb:
 forall G,
- emptyEquiv G = emptyEquiv( emptyEquiv G).
+ emptyEquiv_Hyb G = emptyEquiv_Hyb( emptyEquiv_Hyb G).
 induction G; simpl; auto; destruct a;
 simpl; rewrite <- IHG; auto.
 Qed.
 
-Lemma emptyEquiv_permut_split_last:
+Lemma emptyEquiv_Hyb_permut_split_last:
 forall G C H,
-  G & C ~=~ emptyEquiv H ->
-  emptyEquiv G = G.
+  G & C ~=~ emptyEquiv_Hyb H ->
+  emptyEquiv_Hyb G = G.
 induction G; intros; simpl in *; auto; destruct a; rew_app in *;
 assert (l = nil) by
-  (eapply emptyEquiv_permut_empty; eauto; eapply Mem_here);
-subst; assert (emptyEquiv G = G).
-  assert ((v, nil) :: G & C ~=~ emptyEquiv H) by auto;
-  apply PPermut_split_head in H0; destruct H0 as (l', (hd, (tl, (Ha, Hb))));
+  (eapply emptyEquiv_Hyb_permut_empty; eauto; eapply Mem_here);
+subst; assert (emptyEquiv_Hyb G = G).
+  assert ((v, nil) :: G & C ~=~ emptyEquiv_Hyb H) by auto;
+  apply PPermut_Hyb_split_head in H0; destruct H0 as (l', (hd, (tl, (Ha, Hb))));
   subst; apply permut_nil_eq in Ha; subst.
   rewrite Hb in H1.
   assert (G & C ~=~ hd ++ tl) by
-    ( apply PPermut_last_rev_simpl with (a:=(v,nil));
-      transitivity ((v,nil)::G & C); [ | rewrite H1]; PPermut_simpl).
+    ( apply PPermut_Hyb_last_rev_simpl with (a:=(v,nil));
+      transitivity ((v,nil)::G & C); [ | rewrite H1]; PPermut_Hyb_simpl).
   apply IHG with (C:=C) (H:=hd++tl).
-  rewrite H0. apply PPermut_last_rev_simpl with (a:=(v,nil));
+  rewrite H0. apply PPermut_Hyb_last_rev_simpl with (a:=(v,nil));
   rew_app.
-  assert (hd & (v, nil) ++ tl ~=~ hd ++ tl & (v, nil)) by PPermut_simpl;
+  assert (hd & (v, nil) ++ tl ~=~ hd ++ tl & (v, nil)) by PPermut_Hyb_simpl;
   rewrite <- H2.
-  assert (emptyEquiv (hd ++ tl)&(v, nil) ~=~ emptyEquiv (hd & (v, nil) ++ tl))
-    by (repeat rewrite emptyEquiv_rewrite; PPermut_simpl).
+  assert (emptyEquiv_Hyb (hd ++ tl)&(v, nil) ~=~
+    emptyEquiv_Hyb (hd & (v, nil) ++ tl))
+    by (repeat rewrite emptyEquiv_Hyb_rewrite; PPermut_Hyb_simpl).
   rewrite H3.
   rewrite <- Hb.
-  rewrite <- double_emptyEquiv; auto.
+  rewrite <- double_emptyEquiv_Hyb; auto.
 rewrite H1; auto.
 Qed.
 
-Lemma emptyEquiv_ok_list:
+Lemma emptyEquiv_Hyb_ok_list:
 forall G U,
-  ok_LF G U ->
-  ok_LF (emptyEquiv G) U.
+  ok_Hyb G U ->
+  ok_Hyb (emptyEquiv_Hyb G) U.
 induction G; simpl; intros; auto; destruct a.
 inversion H; subst; constructor; auto.
 Qed.
 
-Lemma emptyEquiv_ok_var:
+Lemma emptyEquiv_Hyb_ok_var:
 forall G U,
-  ok_LF (flat_map snd G) U ->
-  ok_LF (flat_map snd (emptyEquiv G)) U.
+  ok_Hyb (flat_map snd G) U ->
+  ok_Hyb (flat_map snd (emptyEquiv_Hyb G)) U.
 induction G; simpl; intros; auto; destruct a;
 simpl in *; apply IHG.
-eapply ok_LF_split with (G1:=l); eauto.
+eapply ok_Hyb_split with (G1:=l); eauto.
 Qed.
 
-Lemma emptyEquiv_ok_Bg:
+Lemma emptyEquiv_Hyb_ok_Bg_Hyb:
 forall G,
-  ok_Bg G ->
-  ok_Bg (emptyEquiv G).
+  ok_Bg_Hyb G ->
+  ok_Bg_Hyb (emptyEquiv_Hyb G).
 induction G; simpl; intros; auto; destruct a.
-unfold ok_Bg in *;
+unfold ok_Bg_Hyb in *;
 destruct H; split; simpl in *.
 inversion H; subst;
 constructor; auto;
-apply emptyEquiv_ok_list; auto.
-apply emptyEquiv_ok_var.
-apply ok_LF_split in H0; destruct H0; auto.
+apply emptyEquiv_Hyb_ok_list; auto.
+apply emptyEquiv_Hyb_ok_var.
+apply ok_Hyb_split in H0; destruct H0; auto.
 Qed.
 
-Lemma emptyEquiv_ok_list_part:
+Lemma emptyEquiv_Hyb_ok_list_part:
 forall G G' U,
-  ok_LF (G ++ G')  U ->
-  ok_LF ((emptyEquiv G) ++ G') U.
+  ok_Hyb (G ++ G')  U ->
+  ok_Hyb ((emptyEquiv_Hyb G) ++ G') U.
 induction G; simpl; intros; auto; destruct a.
 inversion H; rew_app in *; subst; constructor; auto.
 Qed.
 
-Lemma emptyEquiv_ok_var_part:
+Lemma emptyEquiv_Hyb_ok_var_part:
 forall G G' U,
-  ok_LF (flat_map snd (G++G')) U ->
-  ok_LF (flat_map snd ((emptyEquiv G)++G')) U.
+  ok_Hyb (flat_map snd (G++G')) U ->
+  ok_Hyb (flat_map snd ((emptyEquiv_Hyb G)++G')) U.
 induction G; simpl; intros; auto; destruct a;
 simpl in *; apply IHG.
-eapply ok_LF_split with (G1:=l); rew_app in *; eauto.
+eapply ok_Hyb_split with (G1:=l); rew_app in *; eauto.
 Qed.
 
-Lemma emptyEquiv_ok_Bg_part:
+Lemma emptyEquiv_Hyb_ok_Bg_Hyb_part:
 forall G G',
-  ok_Bg (G ++ G') ->
-  ok_Bg ((emptyEquiv G) ++ G').
+  ok_Bg_Hyb (G ++ G') ->
+  ok_Bg_Hyb ((emptyEquiv_Hyb G) ++ G').
 induction G; simpl; intros; auto; destruct a.
-unfold ok_Bg in *; rew_app in *;
+unfold ok_Bg_Hyb in *; rew_app in *;
 destruct H; split; simpl in *; rew_app.
 inversion H; subst;
 constructor; auto;
-apply emptyEquiv_ok_list_part; auto.
-apply emptyEquiv_ok_var_part.
-apply ok_LF_split in H0; destruct H0; auto.
+apply emptyEquiv_Hyb_ok_list_part; auto.
+apply emptyEquiv_Hyb_ok_var_part.
+apply ok_Hyb_split in H0; destruct H0; auto.
 Qed.
