Hybrid/OkLib.v
@@ -16,125 +16,82 @@ Section Definitions.
 Variables A B : Type.
 
 Inductive ok_Hyb: list (var * A) -> list var -> Prop :=
-| ok_nil: forall U, ok_Hyb nil U
-| ok_step: forall w C G U,
+| ok_Hyb_nil: forall U, ok_Hyb nil U
+| ok_Hyb_step: forall w C G U,
   ~ Mem w U -> ok_Hyb G (w::U) -> ok_Hyb ((w, C)::G) U
 .
 
-(* Copied from standard list, but this one uses List from LibList *)
-Definition flat_map (f:A -> list B) :=
-  fix flat_map (l:list A) : list B :=
-  match l with
-    | nil => nil
-    | x :: t => (f x) ++ (flat_map t)
-  end.
-
-Section FlatMapProp.
-
-Variable f : A -> list B.
-
-Lemma flat_map_nil :
-  flat_map f nil = nil.
-Proof. auto. Qed.
-
-Lemma flat_map_cons : forall x l,
-  flat_map f (x::l) = f x ++ flat_map f l.
-Proof. auto. Qed.
-
-Lemma flat_map_app : forall l1 l2,
-  flat_map f (l1 ++ l2) = flat_map f l1 ++ flat_map f l2.
-Proof.
-induction l1; intros; rew_app; simpl; auto;
-rewrite IHl1; rew_app; auto.
-Qed.
-
-Lemma flat_map_last : forall x l,
-  flat_map f (l & x) = flat_map f l ++ f x.
-Proof. intros; rewrite flat_map_app; simpl; rew_app; auto. Qed.
-
-End FlatMapProp.
-
 End Definitions.
 
-Hint Rewrite flat_map_nil flat_map_cons flat_map_app flat_map_last :
-  rew_flat_map.
-
-Tactic Notation "rew_flat_map" :=
-  autorewrite with rew_flat_map rew_app.
-Tactic Notation "rew_flat_map" "in" hyp(H) :=
-  autorewrite with rew_flat_map rew_app in H.
-Tactic Notation "rew_flat_map" "in" "*" :=
-  autorewrite with rew_flat_map rew_app in *.
-
-Definition ok_Bg_Hyb (G: Background_LF) : Prop :=
+Definition ok_Bg_Hyb (G: bg_Hyb) : Prop :=
 ok_Hyb G nil /\
 ok_Hyb (flat_map snd_ G) nil.
 
-Fixpoint used_t_vars (G: Background_LF) :=
+Fixpoint used_t_vars_Hyb (G: bg_Hyb) :=
 match G with
 | nil => from_list nil
-| (w, Gamma) :: G => from_list (map fst_ Gamma) \u used_t_vars G
+| (w, Gamma) :: G => from_list (map fst_ Gamma) \u used_t_vars_Hyb G
 end.
 
-Fixpoint used_w_vars (G: Background_LF) :=
+Fixpoint used_w_vars_Hyb (G: bg_Hyb) :=
 match G with
 | nil => from_list nil
-| (w, Gamma) :: G => \{w} \u used_w_vars G
+| (w, Gamma) :: G => \{w} \u used_w_vars_Hyb G
 end.
 
 
 (*** Lemmas ***)
 
-Lemma flat_map_ppermut:
+Lemma flat_map_PPermut_Hyb:
 forall G G',
   G ~=~ G' -> flat_map snd_ G *=* flat_map snd_ G'.
 induction G; intros.
-apply PPermut_nil_impl in H; subst; auto.
+apply PPermut_Hyb_nil_impl in H; subst; auto.
 assert (a::G ~=~ G') by auto;
-destruct a; apply PPermut_split_head in H;
+destruct a; apply PPermut_Hyb_split_head in H;
 destruct H as (l', (hd, (tl, (Ha, Hb)))).
 subst; simpl in *.
 specialize IHG with (hd ++ tl).
 rew_flat_map; simpl.
 transitivity (l' ++ flat_map snd_ G); permut_simpl; auto.
 transitivity (flat_map snd_ (hd++tl)).
-apply IHG; apply PPermut_last_rev with (w:=v) (Gamma:=l) (Gamma':=l');
-auto; transitivity ((v,l)::G); PPermut_simpl; rewrite H0; PPermut_simpl.
+apply IHG; apply PPermut_Hyb_last_rev with (w:=v) (Gamma:=l) (Gamma':=l');
+auto; transitivity ((v,l)::G); PPermut_Hyb_simpl; rewrite H0; PPermut_Hyb_simpl.
 rew_flat_map; auto.
 Qed.
 
 (* used_*_vars *)
 
-Lemma used_t_vars_app:
+Lemma used_t_vars_Hyb_app:
 forall x y,
-  used_t_vars (x ++ y) = used_t_vars x \u used_t_vars y.
+  used_t_vars_Hyb (x ++ y) = used_t_vars_Hyb x \u used_t_vars_Hyb y.
 induction x; intros.
 rew_app; simpl; rewrite from_list_nil; rewrite union_empty_l; auto.
 rew_app; destruct a; simpl; rewrite IHx; rewrite union_assoc; auto.
 Qed.
 
-Lemma used_w_vars_app:
+Lemma used_w_vars_Hyb_app:
 forall x y,
-  used_w_vars (x ++ y) = used_w_vars x \u used_w_vars y.
+  used_w_vars_Hyb (x ++ y) = used_w_vars_Hyb x \u used_w_vars_Hyb y.
 induction x; intros.
 rew_app; simpl; rewrite from_list_nil; rewrite union_empty_l; auto.
 rew_app; destruct a; simpl; rewrite IHx; rewrite union_assoc; auto.
 Qed.
 
-Add Morphism used_t_vars: PPermut_used_t.
+Add Morphism used_t_vars_Hyb: PPermut_Hyb_used_t.
 induction x; intros.
-apply PPermut_nil_impl in H; subst; auto.
+apply PPermut_Hyb_nil_impl in H; subst; auto.
 destruct a; simpl.
 assert ((v, l) :: x ~=~ y) by auto.
-apply PPermut_split_head in H;
+apply PPermut_Hyb_split_head in H;
 destruct H as (l', (hd, (tl, (Ha, Hb)))).
 subst.
 assert (x & (v,l) ~=~  (hd ++ tl) & (v, l')).
   transitivity ((v,l)::x); [ | rewrite H0];
-  PPermut_simpl.
-apply PPermut_last_rev in H; auto.
+  PPermut_Hyb_simpl.
+apply PPermut_Hyb_last_rev in H; auto.
 rewrite IHx with (y:=hd ++ tl); auto.
-repeat rewrite used_t_vars_app.
+repeat rewrite used_t_vars_Hyb_app.
 simpl; repeat rewrite <- union_assoc.
 rewrite from_list_nil; rewrite union_empty_l.
 assert (from_list (map fst_ l) = from_list (map fst_ l')).
@@ -142,20 +99,20 @@ assert (from_list (map fst_ l) = from_list (map fst_ l')).
 rewrite union_comm_assoc; rewrite H1; auto.
 Qed.
 
-Add Morphism used_w_vars: PPermut_used_w.
+Add Morphism used_w_vars_Hyb: PPermut_Hyb_used_w.
 induction x; intros.
-apply PPermut_nil_impl in H; subst; auto.
+apply PPermut_Hyb_nil_impl in H; subst; auto.
 destruct a; simpl.
 assert ((v, l) :: x ~=~ y) by auto.
-apply PPermut_split_head in H;
+apply PPermut_Hyb_split_head in H;
 destruct H as (l', (hd, (tl, (Ha, Hb)))).
 subst.
 assert (x & (v,l) ~=~  (hd ++ tl) & (v, l')).
   transitivity ((v,l)::x); [ | rewrite H0];
-  PPermut_simpl.
-apply PPermut_last_rev in H; auto.
+  PPermut_Hyb_simpl.
+apply PPermut_Hyb_last_rev in H; auto.
 rewrite IHx with (y:=hd ++ tl); auto.
-repeat rewrite used_w_vars_app.
+repeat rewrite used_w_vars_Hyb_app.
 simpl; repeat rewrite <- union_assoc.
 rewrite union_comm_assoc;
 rewrite from_list_nil; rewrite union_empty_l.
@@ -204,11 +161,11 @@ Qed.
 
 (* ok_Hyb for a specific type -- would be nice to make it more general btw *)
 
-Add Morphism (@ok_Hyb (list (var*ty))) : ok_Hyb_PPermut_lst_var_ty.
+Add Morphism (@ok_Hyb (list (var*ty))) : ok_Hyb_PPermut_Hyb_lst_var_ty.
 intros x y H; induction H.
 intros; tauto.
 split; intros; inversion H1; subst; constructor; auto;
-apply IHPPermut; auto.
+apply IHPPermut_Hyb; auto.
 split; intros; inversion H1; subst; inversion H7; subst;
 constructor.
 intro; elim H8; rewrite Mem_cons_eq; right; auto.
@@ -222,8 +179,8 @@ constructor.
   subst; elim H8; rewrite Mem_cons_eq; left; auto. auto.
   apply ok_Hyb_used_permut with (U:=w::w'::y0); auto; permut_simpl.
 split; intros.
-  apply IHPPermut2; apply IHPPermut1; auto.
-  apply IHPPermut1; apply IHPPermut2; auto.
+  apply IHPPermut_Hyb2; apply IHPPermut_Hyb1; auto.
+  apply IHPPermut_Hyb1; apply IHPPermut_Hyb2; auto.
 Qed.
 
 Lemma ok_Hyb_permut_any0:
@@ -265,18 +222,18 @@ forall X (G: list (var * X)) G',
 split; intros; [ | symmetry in H]; eapply ok_Hyb_permut_any0; eauto.
 Qed.
 
-Lemma ok_Hyb_PPermut_ty:
+Lemma ok_Hyb_PPermut_Hyb_ty:
 forall G G'
   (H: G ~=~ G'),
   forall U, ok_Hyb (flat_map snd_ G) U <->
   ok_Hyb (flat_map snd_ G') U.
-intros; eapply ok_Hyb_permut_any; apply flat_map_ppermut; auto.
+intros; eapply ok_Hyb_permut_any; apply flat_map_PPermut_Hyb; auto.
 Qed.
 
 Lemma ok_Hyb_fresh_te_list:
 forall G Gamma v A w U,
  ok_Hyb ((w, Gamma) :: G) U ->
- v \notin (used_t_vars ((w,Gamma)::G)) ->
+ v \notin (used_t_vars_Hyb ((w,Gamma)::G)) ->
  ok_Hyb ((w, (v,A)::Gamma) :: G) U.
 intros; inversion H; subst; constructor; auto.
 Qed.
@@ -291,12 +248,12 @@ Qed.
 Lemma ok_Hyb_fresh_te_ty0:
 forall G U w v A,
   ok_Hyb (flat_map snd_ G) U ->
-  v \notin (used_t_vars G \u from_list U) ->
+  v \notin (used_t_vars_Hyb G \u from_list U) ->
   ok_Hyb (flat_map snd_ ((w, (v, A)::nil) :: G)) U.
 induction G; intros.
 simpl in *; constructor; [apply notin_Mem | constructor]; auto.
-eapply ok_Hyb_PPermut_ty with (G':=a:: (w, (v,A)::nil)::G).
-PPermut_simpl. destruct a; simpl in *; rew_app in *.
+eapply ok_Hyb_PPermut_Hyb_ty with (G':=a:: (w, (v,A)::nil)::G).
+PPermut_Hyb_simpl. destruct a; simpl in *; rew_app in *.
 generalize dependent U.
 induction l; intros; simpl in *.
 rew_app in *; apply IHG; eauto.
@@ -312,7 +269,7 @@ Qed.
 Lemma ok_Hyb_fresh_te_ty:
 forall Gamma G U v A w,
  ok_Hyb (flat_map snd_ ((w, Gamma) :: G)) U ->
- v \notin (used_t_vars ((w, Gamma)::G) \u from_list U) ->
+ v \notin (used_t_vars_Hyb ((w, Gamma)::G) \u from_list U) ->
  ok_Hyb (flat_map snd_ ((w, (v, A)::Gamma) :: G)) U.
 intros; simpl in *.
 replace (((v,A) :: Gamma) ++ flat_map snd_ G) with
@@ -323,7 +280,7 @@ Qed.
 Lemma ok_Hyb_fresh_wo_list:
 forall G w U l,
  ok_Hyb G U ->
- w \notin (used_w_vars G)  \u from_list U ->
+ w \notin (used_w_vars_Hyb G)  \u from_list U ->
  ok_Hyb ((w, l) :: G) U.
 induction G; intros.
 constructor.
@@ -350,7 +307,7 @@ Qed.
 Lemma ok_Hyb_fresh_wo_ty:
 forall G w U,
  ok_Hyb (flat_map snd_ G) U ->
- w \notin (used_w_vars G) \u from_list U ->
+ w \notin (used_w_vars_Hyb G) \u from_list U ->
  ok_Hyb (flat_map snd_ ((w, nil) :: G)) U.
 intros; inversion H; subst; simpl in *; rew_app in *; auto.
 Qed.
@@ -358,8 +315,8 @@ Qed.
 Lemma ok_Hyb_fresh_wo_te_list:
 forall U G v A w,
  ok_Hyb G U ->
- w \notin (used_w_vars G) \u from_list U ->
- v \notin (used_t_vars G) ->
+ w \notin (used_w_vars_Hyb G) \u from_list U ->
+ v \notin (used_t_vars_Hyb G) ->
  ok_Hyb ((w, (v,A)::nil) :: G) U.
 intros; apply ok_Hyb_fresh_te_list;
 [ apply ok_Hyb_fresh_wo_list | ]; auto.
@@ -369,8 +326,8 @@ Qed.
 Lemma ok_Hyb_fresh_wo_te_ty:
 forall U G v A w,
  ok_Hyb (flat_map snd_ G) U ->
- w \notin (used_w_vars G) \u from_list U ->
- v \notin (used_t_vars G) \u from_list U ->
+ w \notin (used_w_vars_Hyb G) \u from_list U ->
+ v \notin (used_t_vars_Hyb G) \u from_list U ->
  ok_Hyb (flat_map snd_ ((w, (v,A) :: nil) :: G)) U.
 intros; apply ok_Hyb_fresh_te_ty.
 apply ok_Hyb_fresh_wo_ty; auto.
@@ -396,14 +353,16 @@ Qed.
 
 (* ok_Bg_Hyb *)
 
-Add Morphism ok_Bg_Hyb : ok_Bg_Hyb_PPermut.
+Add Morphism ok_Bg_Hyb : ok_Bg_Hyb_PPermut_Hyb.
 intros; unfold ok_Bg_Hyb; split; intros;
 destruct H0; split;
 [ rewrite <- H | |
-  rewrite H | eapply ok_Hyb_PPermut_ty; try symmetry ]; eauto.
-assert (x ~=~y) by auto; eapply flat_map_ppermut in H; eapply ok_Hyb_PPermut_ty;
+  rewrite H | eapply ok_Hyb_PPermut_Hyb_ty; try symmetry ]; eauto.
+assert (x ~=~y) by auto; eapply flat_map_PPermut_Hyb in H;
+eapply ok_Hyb_PPermut_Hyb_ty;
 try symmetry; eauto.
-assert (x ~=~ y) by auto; eapply flat_map_ppermut in H; eapply ok_Hyb_PPermut_ty;
+assert (x ~=~ y) by auto; eapply flat_map_PPermut_Hyb in H;
+eapply ok_Hyb_PPermut_Hyb_ty;
 eauto.
 Qed.
 
@@ -421,7 +380,7 @@ forall G Ctx Ctx' w,
   ok_Bg_Hyb ((w, Ctx) :: G) ->
   ok_Bg_Hyb ((w, Ctx') :: G).
 intros;
-assert ((w, Ctx) :: G ~=~ (w, Ctx') :: G) by PPermut_simpl;
+assert ((w, Ctx) :: G ~=~ (w, Ctx') :: G) by PPermut_Hyb_simpl;
 rewrite <- H1; auto.
 Qed.
 
@@ -431,14 +390,14 @@ forall G Ctx Ctx' w,
   ok_Bg_Hyb (G ++ (w, Ctx) :: nil) ->
   ok_Bg_Hyb (G ++ (w, Ctx') :: nil).
 intros;
-assert (G & (w, Ctx) ~=~ G & (w, Ctx')) by PPermut_simpl;
+assert (G & (w, Ctx) ~=~ G & (w, Ctx')) by PPermut_Hyb_simpl;
 rewrite <- H1; auto.
 Qed.
 
 Lemma ok_Bg_Hyb_fresh_te:
 forall G Gamma v A w,
  ok_Bg_Hyb ((w, Gamma) :: G) ->
- v \notin (used_t_vars ((w,Gamma)::G)) ->
+ v \notin (used_t_vars_Hyb ((w,Gamma)::G)) ->
  ok_Bg_Hyb ((w, (v,A)::Gamma) :: G).
 intros; unfold ok_Bg_Hyb in *;  destruct H; split;
 [ apply ok_Hyb_fresh_te_list |
@@ -449,7 +408,7 @@ Qed.
 Lemma ok_Bg_Hyb_fresh_wo:
 forall G w,
  ok_Bg_Hyb G ->
- w \notin (used_w_vars G) ->
+ w \notin (used_w_vars_Hyb G) ->
  ok_Bg_Hyb ((w, nil) :: G).
 intros; unfold ok_Bg_Hyb in *;  destruct H; split;
 [ eapply ok_Hyb_fresh_wo_list |
@@ -460,8 +419,8 @@ Qed.
 Lemma ok_Bg_Hyb_fresh_wo_te:
 forall G w v A,
  ok_Bg_Hyb G ->
- w \notin (used_w_vars G) ->
- v \notin (used_t_vars G) ->
+ w \notin (used_w_vars_Hyb G) ->
+ v \notin (used_t_vars_Hyb G) ->
  ok_Bg_Hyb ((w, (v, A) :: nil) :: G).
 intros; unfold ok_Bg_Hyb in *;  destruct H; split;
 [ apply ok_Hyb_fresh_wo_te_list |
@@ -472,7 +431,7 @@ Qed.
 Lemma ok_Bg_Hyb_cons_last:
 forall G a,
   ok_Bg_Hyb (G & a) <-> ok_Bg_Hyb (a :: G).
-intros; assert (G & a ~=~ a :: G) by PPermut_simpl;
+intros; assert (G & a ~=~ a :: G) by PPermut_Hyb_simpl;
 rewrite H; split; auto.
 Qed.
 
@@ -480,12 +439,12 @@ Lemma ok_Bg_Hyb_swap:
 forall C C' G,
   ok_Bg_Hyb (C :: G & C') ->
   ok_Bg_Hyb (C' :: G & C).
-intros; assert (C:: G & C' ~=~ C' :: G & C) by PPermut_simpl;
+intros; assert (C:: G & C' ~=~ C' :: G & C) by PPermut_Hyb_simpl;
 rewrite <- H0; auto.
 Qed.
 
 Hint Resolve ok_Bg_Hyb_cons_last ok_Bg_Hyb_swap.
-Hint Resolve ok_Bg_Hyb_permut_last: ok_bg_rew.
+Hint Resolve ok_Bg_Hyb_permut_last: ok_bg_hyb_rew.
 Hint Resolve ok_Bg_Hyb_fresh_te ok_Bg_Hyb_fresh_wo ok_Bg_Hyb_fresh_wo_te.
 
 Lemma ok_Bg_Hyb_permut_first_tail:
@@ -494,13 +453,13 @@ forall G C C' w x A,
   C *=* (x,A)::C' ->
   ok_Bg_Hyb ((w, C') :: G).
 intros;
-assert ((w,(x, A) :: C') :: G ~=~ (w, C) :: G) by PPermut_simpl;
+assert ((w,(x, A) :: C') :: G ~=~ (w, C) :: G) by PPermut_Hyb_simpl;
 rewrite <- H1 in H; unfold ok_Bg_Hyb in *; destruct H; split; simpl in *.
 inversion H; subst; constructor; auto.
 rew_app in *; inversion H2; subst; simpl in *.
 apply ok_Hyb_used_weakening with (x:=x); auto.
 Qed.
-Hint Resolve ok_Bg_Hyb_permut_first_tail : ok_bg_rew.
+Hint Resolve ok_Bg_Hyb_permut_first_tail : ok_bg_hyb_rew.
 
 Lemma ok_Bg_Hyb_empty_first:
 forall w G Gamma,
@@ -511,7 +470,7 @@ intros; unfold ok_Bg_Hyb; destruct H; split;
  eapply ok_Hyb_empty_first_ty]; eauto.
 Qed.
 
-Hint Resolve ok_Bg_Hyb_empty_first : ok_bg_rew.
+Hint Resolve ok_Bg_Hyb_empty_first : ok_bg_hyb_rew.
 
 Lemma ok_Bg_Hyb_Mem_eq:
 forall w C C' v A A0 G,
@@ -528,7 +487,8 @@ assert (C *=* (v, A) :: (v, A0) :: gh ++ gt) by (rewrite H0; permut_simpl);
 unfold ok_Bg_Hyb in *; destruct H.
 assert (ok_Hyb (flat_map snd_ ((w, (v, A) :: (v, A0) :: gh ++ gt ) :: G )) nil)
 by
-  (apply ok_Hyb_PPermut_ty with (G := ((w, C) :: G)); [PPermut_simpl | auto]).
+  (apply ok_Hyb_PPermut_Hyb_ty with (G := ((w, C) :: G));
+   [PPermut_Hyb_simpl | auto]).
 simpl in *. rew_app in *; inversion H4; subst.
 inversion H10; subst;
 elim H11; apply Mem_here.
@@ -546,7 +506,7 @@ apply permut_Mem_split_head with (l2 := C) in H0; auto;
 destruct H0 as (gh); destruct H0 as (gt); subst.
 assert ((w, gh & (v, A) ++ gt) :: G' & (w', (v, A') :: C') ~=~
         (w, (v, A) :: gh ++ gt) :: (w', (v, A') :: C') :: G') by
-(PPermut_simpl; apply PPermut_skip; [permut_simpl | auto]).
+(PPermut_Hyb_simpl; apply PPermut_Hyb_skip; [permut_simpl | auto]).
 rewrite H0 in H; unfold ok_Bg_Hyb in H; destruct H.
 rew_flat_map in *. simpl ok_Hyb in H2.
 rew_app in *. inversion H2; subst.
@@ -561,12 +521,12 @@ forall G w C v A,
   ok_Bg_Hyb (G & (w, (v,A) :: C)) ->
   ok_Bg_Hyb (G & (w, C)).
 intros;
-assert (G & (w, C) ~=~ (w,C) :: G) by PPermut_simpl;
-assert (G & (w, (v, A) :: C) ~=~ (w, (v,A) :: C) :: G) by PPermut_simpl;
+assert (G & (w, C) ~=~ (w,C) :: G) by PPermut_Hyb_simpl;
+assert (G & (w, (v, A) :: C) ~=~ (w, (v,A) :: C) :: G) by PPermut_Hyb_simpl;
 rewrite H1 in H; destruct H; simpl in *; split; rew_app in *.
 inversion H; subst; rewrite H0; constructor; auto.
 inversion H2; subst;
-apply ok_Hyb_PPermut_ty with (U:=nil) in H0;
+apply ok_Hyb_PPermut_Hyb_ty with (U:=nil) in H0;
 apply H0; simpl;
 apply ok_Hyb_used_weakening in H8;
 auto.
@@ -577,7 +537,8 @@ forall G w C C0 v A,
   ok_Bg_Hyb (C0::G & (w, (v,A) :: C)) ->
   ok_Bg_Hyb (C0::G & (w, C)).
 intros;
-assert (C0 :: G & (w, C)  ~=~ (C0 :: G) & (w, C)) by (rew_app; PPermut_simpl);
+assert (C0 :: G & (w, C)  ~=~ (C0 :: G) & (w, C))
+  by (rew_app; PPermut_Hyb_simpl);
 rewrite H0; eapply ok_Bg_Hyb_permut_no_last; rew_app; eauto.
 Qed.
 
@@ -585,7 +546,7 @@ Lemma ok_Bg_Hyb_no_last:
 forall G C,
   ok_Bg_Hyb (G & C) -> ok_Bg_Hyb G.
 intros;
-assert (G & C ~=~ (C :: nil) ++ G) by PPermut_simpl; rewrite H0 in H;
+assert (G & C ~=~ (C :: nil) ++ G) by PPermut_Hyb_simpl; rewrite H0 in H;
 destruct H; split.
 eapply ok_Hyb_split with (G1:=C::nil) (G2:=G); eauto.
 destruct C; rew_app in *; simpl in *.
@@ -598,11 +559,11 @@ forall G w C C0 v A,
   ok_Bg_Hyb (G & (w, (v,A) :: C) & C0) ->
   ok_Bg_Hyb (G & (w, C) & C0).
 intros.
-assert (G & (w, C) & C0 ~=~ G & C0 & (w, C)) by PPermut_simpl;
+assert (G & (w, C) & C0 ~=~ G & C0 & (w, C)) by PPermut_Hyb_simpl;
 rewrite H0;
 apply ok_Bg_Hyb_permut_no_last with (v:=v) (A:=A).
 assert (G & C0 & (w, (v, A) :: C) ~=~ G & (w, (v, A) :: C) & C0)
-  by PPermut_simpl;
+  by PPermut_Hyb_simpl;
 rewrite H1; auto.
 Qed.
 
@@ -611,7 +572,8 @@ forall w w' C C' G,
   ok_Bg_Hyb ((w, C) :: G & (w', C')) ->
   w <> w'.
 intros.
-assert ((w, C) :: G & (w', C') ~=~ (w, C) :: (w', C') :: G) by PPermut_simpl;
+assert ((w, C) :: G & (w', C') ~=~ (w, C) :: (w', C') :: G)
+  by PPermut_Hyb_simpl;
 rewrite H0 in H;
 destruct H; simpl in *. inversion H; subst; inversion H7; subst.
 rewrite Mem_cons_eq in H8. rewrite Mem_nil_eq in H8. auto.
@@ -622,7 +584,7 @@ forall w w' C C' G,
   ok_Bg_Hyb (G & (w, C) & (w', C')) ->
   w <> w'.
 intros;
-assert (G & (w, C) & (w', C') ~=~ (w, C) :: (w', C') :: G) by PPermut_simpl;
+assert (G & (w, C) & (w', C') ~=~ (w, C) :: (w', C') :: G) by PPermut_Hyb_simpl;
 rewrite H0 in H;
 destruct H; simpl in *; inversion H; subst; inversion H7; subst.
 rewrite Mem_cons_eq in H8. rewrite Mem_nil_eq in H8; auto.
@@ -633,9 +595,9 @@ forall G w w' C C',
   ok_Bg_Hyb (G & (w, C) & (w', C')) ->
   ok_Bg_Hyb (G & (w', C) & (w, C')).
 intros.
-assert (G & (w, C) & (w', C') ~=~ (w, C) :: (w', C') :: G) by PPermut_simpl.
+assert (G & (w, C) & (w', C') ~=~ (w, C) :: (w', C') :: G) by PPermut_Hyb_simpl.
 rewrite H0 in H.
-assert (G & (w', C) & (w, C') ~=~ (w', C) :: (w, C') :: G) by PPermut_simpl.
+assert (G & (w', C) & (w, C') ~=~ (w', C) :: (w, C') :: G) by PPermut_Hyb_simpl.
 rewrite H1.
 destruct H; split; simpl in *.
 inversion H; subst; constructor. rewrite Mem_nil_eq; tauto.
@@ -654,37 +616,35 @@ forall G G' w C C',
 unfold ok_Bg_Hyb.
 intros. destruct H.
 assert ((w,C) :: G ~=~ (w, C') :: G').
-  transitivity (G & (w,C)); [ | rewrite H0]; PPermut_simpl.
-apply PPermut_split_head in H2.
+  transitivity (G & (w,C)); [ | rewrite H0]; PPermut_Hyb_simpl.
+apply PPermut_Hyb_split_head in H2.
 destruct H2 as (C'', (hd, (tl, (H2, H3)))).
 assert ((w, C') :: G' = hd & (w, C'') ++ tl) by auto.
 apply cons_eq_last_val_app_inv in H4; destruct H4.
 (* case 1: positive - hd = nil and C *=* C'' *)
 destruct H4; destruct H5; subst; rew_app in *;
 inversion H3; subst; split; auto;
-apply PPermut_last_rev with (Gamma:=C)(Gamma':=C'')(w:=w); auto.
+apply PPermut_Hyb_last_rev with (Gamma:=C)(Gamma':=C'')(w:=w); auto.
 (* case 2: negative *)
 destruct H4 as (hd', H4); subst.
 assert ((w, C) :: G ~=~ (w, C') :: (w, C'') :: hd' ++ tl).
-  transitivity (G & (w,C)). PPermut_simpl.
+  transitivity (G & (w,C)). PPermut_Hyb_simpl.
   rewrite H0; transitivity ((w, C') :: G'); [ | rewrite H3];
-  PPermut_simpl.
+  PPermut_Hyb_simpl.
 rewrite H4 in H; inversion H; subst; inversion H10; subst.
 elim H11; apply Mem_here.
 Qed.
 
-
 (* FIXME: generalize all the ok_Bg_Hyb_split* into :
    ok_Bg_Hyb G <- ok_Bg_Hyb reorder_G <- ok_Bg_Hyb reorder_G' <- ok_Bg_Hyb G':
    reorder X ~=~ X and all the singletons are in the front *)
-
 
 Lemma ok_Bg_Hyb_split1:
 forall G w w' C C',
   ok_Bg_Hyb ((w,C)::G & (w',C')) ->
   ok_Bg_Hyb ((w, C ++ C') :: G).
 intros.
-assert ((w, C) :: G & (w', C') ~=~ (w,C) :: (w', C')::G) by PPermut_simpl.
+assert ((w, C) :: G & (w', C') ~=~ (w,C) :: (w', C')::G) by PPermut_Hyb_simpl.
 rewrite H0 in H; destruct H; split; simpl in *.
 inversion H; subst; inversion H7; subst; constructor; auto;
 apply ok_Hyb_used_weakening with (x:=w'); auto.
@@ -696,7 +656,7 @@ forall G w w' C C',
   ok_Bg_Hyb ((w,C)::G & (w',C')) ->
   ok_Bg_Hyb ((w', C' ++ C) :: G).
 intros.
-assert ((w, C) :: G & (w', C') ~=~ (w', C') :: (w, C)::G) by PPermut_simpl.
+assert ((w, C) :: G & (w', C') ~=~ (w', C') :: (w, C)::G) by PPermut_Hyb_simpl.
 rewrite H0 in H; destruct H; split; simpl in *.
 inversion H; subst; inversion H7; subst;
 constructor; auto.
@@ -710,9 +670,9 @@ forall G w w' w'' C C' C'',
   ok_Bg_Hyb ((w, C) :: G & (w', C' ++ C'')).
 intros.
 assert ((w, C) :: G & (w', C') & (w'',C'') ~=~
-  (w, C) :: (w', C'):: (w'',C'') :: G) by PPermut_simpl.
+  (w, C) :: (w', C'):: (w'',C'') :: G) by PPermut_Hyb_simpl.
 assert ((w,C) :: G & (w', C'++C'') ~=~ (w,C) :: (w', C'++C'') :: G)
-  by PPermut_simpl.
+  by PPermut_Hyb_simpl.
 rewrite H0 in H; rewrite H1; destruct H; split; simpl in *.
 inversion H; subst; inversion H8; subst; inversion H10; subst;
 constructor; auto; constructor; auto.
@@ -726,17 +686,17 @@ forall G w w' C C',
   ok_Bg_Hyb (G & (w', C' ++ C)).
 intros.
 assert (G & (w, C) & (w', C') ~=~
-  (w, C) :: (w', C') :: G) by PPermut_simpl.
+  (w, C) :: (w', C') :: G) by PPermut_Hyb_simpl.
 assert (G & (w', C'++C) ~=~ (w', C'++C) :: G)
-  by PPermut_simpl.
+  by PPermut_Hyb_simpl.
 rewrite H0 in H; rewrite H1; destruct H; split.
 simpl in *; inversion H; subst; inversion H8; subst; constructor; auto.
 rewrite Mem_nil_eq; tauto.
 apply ok_Hyb_used_weakening with (x:=w);
 apply ok_Hyb_used_permut with (U:= w'::w::nil);
 try permut_simpl; auto.
-assert ((w', C'++C)::G ~=~ (w',C++C')::G) by PPermut_simpl.
-apply ok_Hyb_PPermut_ty with (U:=nil) in H3.
+assert ((w', C'++C)::G ~=~ (w',C++C')::G) by PPermut_Hyb_simpl.
+apply ok_Hyb_PPermut_Hyb_ty with (U:=nil) in H3.
 simpl in *; rew_app in *.
 apply H3. auto.
 Qed.
@@ -747,9 +707,9 @@ forall G w w' C C',
   ok_Bg_Hyb (G & (w, C ++ C')).
 intros.
 assert (G & (w, C) & (w', C') ~=~
-  (w, C) :: (w', C') :: G) by PPermut_simpl.
+  (w, C) :: (w', C') :: G) by PPermut_Hyb_simpl.
 assert (G & (w, C++C') ~=~ (w, C++C') :: G)
-  by PPermut_simpl.
+  by PPermut_Hyb_simpl.
 rewrite H0 in H; rewrite H1; destruct H; split; simpl in *.
 inversion H; subst; inversion H8; subst.
 constructor; auto;
@@ -763,9 +723,9 @@ forall G w C C' C'' w' w'',
   ok_Bg_Hyb (G & (w, C ++ C') & (w'', C'')).
 intros.
 assert (G & (w,C) & (w', C') & (w'',C'') ~=~
-  (w, C) :: (w', C'):: (w'',C'') :: G) by PPermut_simpl.
+  (w, C) :: (w', C'):: (w'',C'') :: G) by PPermut_Hyb_simpl.
 assert (G & (w, C++C') & (w'', C'') ~=~ (w, C ++ C') :: (w'', C'') :: G)
-  by PPermut_simpl.
+  by PPermut_Hyb_simpl.
 rewrite H0 in H; rewrite H1; destruct H; split; simpl in *.
 inversion H; subst; inversion H8; subst; inversion H10; subst.
 constructor; auto.
@@ -773,23 +733,16 @@ apply ok_Hyb_used_weakening with (x:=w'); auto.
 rew_app; auto.
 Qed.
 
-(* This is actually false
-Lemma ok_Bg_Hyb_split7:
-forall G w w' w'' C C' C'',
-  ok_Bg_Hyb ((w,C)::G & (w'',C'')) ->
-  ok_Bg_Hyb ((w, C ++ C'') :: G & (w', C')).
-*)
-
 Lemma ok_Bg_Hyb_split8:
 forall G G' w w' w'' C C' C'',
   ok_Bg_Hyb (G ++ G' ++ (w, C) :: (w', C') :: (w'', C'') :: nil) ->
   ok_Bg_Hyb (G ++ G' ++ (w', C') :: (w'', C'' ++ C)::nil) .
 intros.
 assert (G++G' ++ (w, C) :: (w', C') :: (w'',C'') :: nil ~=~
-  (w, C) :: (w', C'):: (w'',C'') :: G ++ G') by PPermut_simpl.
+  (w, C) :: (w', C'):: (w'',C'') :: G ++ G') by PPermut_Hyb_simpl.
 assert (G ++ G' ++ (w', C') :: (w'', C'' ++ C) :: nil ~=~
   (w', C') :: (w'', C''++C) :: G ++ G')
-  by PPermut_simpl.
+  by PPermut_Hyb_simpl.
 rewrite H0 in H; rewrite H1; destruct H; split.
 simpl in *.
 inversion H; subst; inversion H8; subst; inversion H10; subst.
@@ -803,10 +756,11 @@ contradiction.
 apply ok_Hyb_used_weakening with (x:=w);
 apply ok_Hyb_used_permut with (U:=w'' :: w' :: w :: nil);
 auto; permut_simpl.
-apply ok_Hyb_PPermut_ty with (G':=(w',C') :: (w'', C'')::(w,C) :: G ++ G') in H2.
+apply ok_Hyb_PPermut_Hyb_ty with
+  (G':=(w',C') :: (w'', C'')::(w,C) :: G ++ G') in H2.
 simpl in *.
 rew_app. auto.
-PPermut_simpl.
+PPermut_Hyb_simpl.
 Qed.
 
 Lemma ok_Bg_Hyb_split9:
@@ -815,10 +769,10 @@ forall G w w' w'' C C' C'',
   ok_Bg_Hyb ((w, C++C') :: G & (w'', C'')).
 intros.
 assert ((w, C) :: G & (w', C') & (w'',C'') ~=~
-  (w, C) :: (w', C'):: (w'',C'') :: G) by PPermut_simpl.
+  (w, C) :: (w', C'):: (w'',C'') :: G) by PPermut_Hyb_simpl.
 assert ((w, C++C') :: G & (w'', C'')  ~=~
   (w, C++C') :: (w'', C'') :: G)
-  by PPermut_simpl.
+  by PPermut_Hyb_simpl.
 rewrite H0 in H; rewrite H1; destruct H; split; simpl in *.
 inversion H; subst; inversion H8; subst; inversion H10; subst.
 constructor; auto; constructor.
@@ -837,9 +791,9 @@ forall G G' w1 w2 w3 w4 c1 c2 c3 c4,
   ok_Bg_Hyb (G ++ (w1, c1)::G' ++ (w2, c2 ++ c3) :: (w4, c4) :: nil).
 intros.
 assert (G ++ (w1,c1) :: G' ++ (w2, c2) :: (w3, c3) :: (w4,c4) :: nil ~=~
-   (w1,c1) :: (w2, c2) :: (w3, c3) :: (w4,c4) :: G ++ G') by PPermut_simpl.
+   (w1,c1) :: (w2, c2) :: (w3, c3) :: (w4,c4) :: G ++ G') by PPermut_Hyb_simpl.
 assert (G ++ (w1, c1) :: G' ++ (w2, c2 ++ c3) :: (w4, c4) :: nil~=~
-   (w1,c1) :: (w2, c2 ++ c3) :: (w4,c4) :: G ++ G') by PPermut_simpl.
+   (w1,c1) :: (w2, c2 ++ c3) :: (w4,c4) :: G ++ G') by PPermut_Hyb_simpl.
 rewrite H0 in H; rewrite H1; destruct H; split; simpl in *.
 inversion H; subst; inversion H8; subst; inversion H10; subst;
 inversion H12; subst.
@@ -857,10 +811,10 @@ Qed.
 
 Hint Resolve ok_Bg_Hyb_split1 ok_Bg_Hyb_split2 ok_Bg_Hyb_split3 ok_Bg_Hyb_split4
   ok_Bg_Hyb_split5 ok_Bg_Hyb_split6 ok_Bg_Hyb_split8
-  ok_Bg_Hyb_split9 ok_Bg_Hyb_split10 : ok_bg_rew.
+  ok_Bg_Hyb_split9 ok_Bg_Hyb_split10 : ok_bg_hyb_rew.
 Hint Resolve ok_Bg_Hyb_permut_no_last ok_Bg_Hyb_permut_no_last_spec2
   ok_Bg_Hyb_permut_no_last_spec ok_Bg_Hyb_first_last_neq
-  ok_Bg_Hyb_last_last2_neq : ok_bg_rew.
+  ok_Bg_Hyb_last_last2_neq : ok_bg_hyb_rew.
 Hint Resolve ok_Bg_Hyb_swap_worlds.
 
 Close Scope permut_scope.
