Hybrid/PPermutLib.v
@@ -6,63 +6,63 @@ Require Export PermutLib.
 
 Open Scope permut_scope.
 
-Inductive PPermut_LF: list Context_LF -> list Context_LF -> Prop :=
-| PPermut_LF_nil: PPermut_LF nil nil
-| PPermut_LF_skip: forall G G' w Gamma Gamma',
+Inductive PPermut_Hyb: list ctx_Hyb -> list ctx_Hyb -> Prop :=
+| PPermut_Hyb_nil: PPermut_Hyb nil nil
+| PPermut_Hyb_skip: forall G G' w Gamma Gamma',
     Gamma *=* Gamma' ->
-    PPermut_LF G G' ->
-    PPermut_LF ((w, Gamma)::G) ((w,Gamma')::G')
-| PPermut_LF_swap: forall G w w' Gamma0 Gamma0' Gamma1 Gamma1',
+    PPermut_Hyb G G' ->
+    PPermut_Hyb ((w, Gamma)::G) ((w,Gamma')::G')
+| PPermut_Hyb_swap: forall G w w' Gamma0 Gamma0' Gamma1 Gamma1',
     Gamma0 *=* Gamma1 ->
     Gamma0' *=* Gamma1' ->
-    PPermut_LF ((w, Gamma0) :: (w', Gamma0') :: G)
+    PPermut_Hyb ((w, Gamma0) :: (w', Gamma0') :: G)
                 ((w', Gamma1') :: (w, Gamma1) :: G)
-| PPermut_LF_trans: forall G G' G'',
-    PPermut_LF G G' -> PPermut_LF G' G'' -> PPermut_LF G G''.
-Hint Resolve PPermut_LF_nil PPermut_LF_skip PPermut_LF_swap.
-Hint Constructors PPermut_LF : ppermut_rew.
+| PPermut_Hyb_trans: forall G G' G'',
+    PPermut_Hyb G G' -> PPermut_Hyb G' G'' -> PPermut_Hyb G G''.
+Hint Resolve PPermut_Hyb_nil PPermut_Hyb_skip PPermut_Hyb_swap.
+Hint Constructors PPermut_Hyb : ppermut_rew.
 
-Notation "G ~=~ G'" := (PPermut_LF G G') (at level 70) : permut_scope.
+Notation "G ~=~ G'" := (PPermut_Hyb G G') (at level 70) : permut_scope.
 
-Lemma PPermut_LF_reflexive:
-  Reflexive PPermut_LF.
+Lemma PPermut_Hyb_reflexive:
+  Reflexive PPermut_Hyb.
 unfold Reflexive; intros;
 induction x; [ | destruct a]; eauto.
 Qed.
 
-Lemma PPermut_LF_symmetric:
-  Symmetric PPermut_LF.
+Lemma PPermut_Hyb_symmetric:
+  Symmetric PPermut_Hyb.
 unfold Symmetric; intros;
 induction H; eauto with ppermut_rew.
-  apply PPermut_LF_trans with (G':=(w, Gamma')::G); eauto with ppermut_rew;
-  apply PPermut_LF_skip;
+  apply PPermut_Hyb_trans with (G':=(w, Gamma')::G); eauto with ppermut_rew;
+  apply PPermut_Hyb_skip;
   [ apply permut_sym |
-    apply PPermut_LF_reflexive];
+    apply PPermut_Hyb_reflexive];
   auto.
-  apply PPermut_LF_swap; apply permut_sym; assumption.
+  apply PPermut_Hyb_swap; apply permut_sym; assumption.
 Qed.
 
-Lemma PPermut_LF_transitive:
-  Transitive PPermut_LF.
-exact PPermut_LF_trans.
+Lemma PPermut_Hyb_transitive:
+  Transitive PPermut_Hyb.
+exact PPermut_Hyb_trans.
 Qed.
-Hint Resolve PPermut_LF_reflexive PPermut_LF_symmetric.
+Hint Resolve PPermut_Hyb_reflexive PPermut_Hyb_symmetric.
 
-Theorem PPermut_LF'oid: Setoid_Theory _ PPermut_LF.
+Theorem PPermut_Hyb'oid: Setoid_Theory _ PPermut_Hyb.
   split.
-  exact PPermut_LF_reflexive.
-  exact PPermut_LF_symmetric.
-  exact PPermut_LF_transitive.
+  exact PPermut_Hyb_reflexive.
+  exact PPermut_Hyb_symmetric.
+  exact PPermut_Hyb_transitive.
 Qed.
 
-Add Setoid (list Context_LF) PPermut_LF PPermut_LF'oid as PPermut_LFoid.
+Add Setoid (list ctx_Hyb) PPermut_Hyb PPermut_Hyb'oid as PPermut_Hyboid.
 
-Add Morphism (@cons Context_LF) : PPermut_LF_cons.
+Add Morphism (@cons ctx_Hyb) : PPermut_Hyb_cons.
 intro y; destruct y; auto.
 Qed.
-Hint Resolve PPermut_LF_cons.
+Hint Resolve PPermut_Hyb_cons.
 
-Lemma PPermut_LF_app_tail:
+Lemma PPermut_Hyb_app_tail:
 forall G G' G0,
   G ~=~ G' ->
   G ++ G0 ~=~ G' ++ G0.
@@ -70,22 +70,22 @@ intros; induction H; simpl; rew_app; auto;
 econstructor; eauto.
 Qed.
 
-Lemma PPermut_LF_app_head:
+Lemma PPermut_Hyb_app_head:
 forall G0 G G',
   G ~=~ G' ->
   G0 ++ G ~=~ G0 ++ G'.
 intros; induction G0; simpl; rew_app; auto.
 Qed.
-Hint Resolve PPermut_LF_app_tail PPermut_LF_app_head.
+Hint Resolve PPermut_Hyb_app_tail PPermut_Hyb_app_head.
 
-Add Morphism (@append Context_LF) : PPermut_LF_app.
+Add Morphism (@append ctx_Hyb) : PPermut_Hyb_app.
 intros; induction H; simpl in *; rew_app; auto.
 transitivity ((w, Gamma0) :: (w', Gamma0') :: G ++ y0); auto.
 transitivity (G' ++ y0); auto.
 Qed.
-Hint Resolve PPermut_LF_app.
+Hint Resolve PPermut_Hyb_app.
 
-Theorem PPermut_LF_app_comm:
+Theorem PPermut_Hyb_app_comm:
 forall G1 G2,
   G1 ++ G2 ~=~ G2 ++ G1.
 induction G1; intros; simpl; rew_app;
@@ -99,85 +99,85 @@ transitivity ((v,l) :: (v0, l0) :: G2 ++ G1);
 rew_app; constructor; auto;
 transitivity ((v,l) :: G1 ++ G2); auto.
 Qed.
-Hint Resolve PPermut_LF_app_comm.
+Hint Resolve PPermut_Hyb_app_comm.
 
 
 (*** Automation **)
 (* Based on permutation tactics from tlc's LibListSorted *)
 
-Lemma PPermut_LF_get_1 : forall l1 l2,
-  PPermut_LF (l1 ++ l2) (l1 ++ l2).
+Lemma PPermut_Hyb_get_1 : forall l1 l2,
+  PPermut_Hyb (l1 ++ l2) (l1 ++ l2).
 auto.
 Qed.
 
-Lemma PPermut_LF_get_2 : forall l1 l2 l3,
-  PPermut_LF (l1 ++ l2 ++ l3) (l2 ++ l1 ++ l3).
+Lemma PPermut_Hyb_get_2 : forall l1 l2 l3,
+  PPermut_Hyb (l1 ++ l2 ++ l3) (l2 ++ l1 ++ l3).
 intros;
 assert (l1 ++ l2 ~=~ l2 ++ l1) as H by auto;
 transitivity ((l1 ++ l2) ++ l3); [ | rewrite H ]; rew_app; auto.
 Qed.
 
-Lemma PPermut_LF_get_3 : forall l1 l2 l3 l4,
-  PPermut_LF (l1 ++ l2 ++ l3 ++ l4) (l2 ++ l3 ++ l1 ++ l4).
+Lemma PPermut_Hyb_get_3 : forall l1 l2 l3 l4,
+  PPermut_Hyb (l1 ++ l2 ++ l3 ++ l4) (l2 ++ l3 ++ l1 ++ l4).
 intros;
-do 2 rewrite <- (@app_assoc _ l2); eapply PPermut_LF_get_2.
+do 2 rewrite <- (@app_assoc _ l2); eapply PPermut_Hyb_get_2.
 Qed.
 
-Lemma PPermut_LF_get_4 : forall l1 l2 l3 l4 l5,
-  PPermut_LF (l1 ++ l2 ++ l3 ++ l4 ++ l5)
+Lemma PPermut_Hyb_get_4 : forall l1 l2 l3 l4 l5,
+  PPermut_Hyb (l1 ++ l2 ++ l3 ++ l4 ++ l5)
          (l2 ++ l3 ++ l4 ++ l1 ++ l5).
 intros;
-do 2 rewrite <- (@app_assoc _ l2); eapply PPermut_LF_get_3.
+do 2 rewrite <- (@app_assoc _ l2); eapply PPermut_Hyb_get_3.
 Qed.
 
-Lemma PPermut_LF_get_5 : forall l1 l2 l3 l4 l5 l6,
-  PPermut_LF (l1 ++ l2 ++ l3 ++ l4 ++ l5 ++ l6)
+Lemma PPermut_Hyb_get_5 : forall l1 l2 l3 l4 l5 l6,
+  PPermut_Hyb (l1 ++ l2 ++ l3 ++ l4 ++ l5 ++ l6)
          (l2 ++ l3 ++ l4 ++ l5 ++ l1 ++ l6).
 intros;
-do 2 rewrite <- (@app_assoc _ l2); eapply PPermut_LF_get_4.
+do 2 rewrite <- (@app_assoc _ l2); eapply PPermut_Hyb_get_4.
 Qed.
 
-Lemma PPermut_LF_get_6 : forall l1 l2 l3 l4 l5 l6 l7,
-  PPermut_LF (l1 ++ l2 ++ l3 ++ l4 ++ l5 ++ l6 ++ l7)
+Lemma PPermut_Hyb_get_6 : forall l1 l2 l3 l4 l5 l6 l7,
+  PPermut_Hyb (l1 ++ l2 ++ l3 ++ l4 ++ l5 ++ l6 ++ l7)
          (l2 ++ l3 ++ l4 ++ l5 ++ l6 ++ l1 ++ l7).
 intros;
-do 2 rewrite <- (@app_assoc _ l2); eapply PPermut_LF_get_5.
+do 2 rewrite <- (@app_assoc _ l2); eapply PPermut_Hyb_get_5.
 Qed.
 
-Lemma PPermut_LF_tactic_setup : forall l1 l2,
-  PPermut_LF (nil ++ l1 ++ nil) (l2 ++ nil) -> PPermut_LF l1 l2.
+Lemma PPermut_Hyb_tactic_setup : forall l1 l2,
+  PPermut_Hyb (nil ++ l1 ++ nil) (l2 ++ nil) -> PPermut_Hyb l1 l2.
 intros; rew_app in *; auto.
 Qed.
 
-Lemma PPermut_LF_tactic_keep : forall l1 l2 l3 l4,
-  PPermut_LF ((l1 ++ l2) ++ l3) l4 ->
-  PPermut_LF (l1 ++ (l2 ++ l3)) l4.
+Lemma PPermut_Hyb_tactic_keep : forall l1 l2 l3 l4,
+  PPermut_Hyb ((l1 ++ l2) ++ l3) l4 ->
+  PPermut_Hyb (l1 ++ (l2 ++ l3)) l4.
 intros; rew_app in *; auto.
 Qed.
 
-Lemma PPermut_LF_tactic_simpl : forall l1 l2 l3 l4,
-  PPermut_LF (l1 ++ l3) l4 ->
-  PPermut_LF (l1 ++ (l2 ++ l3)) (l2 ++ l4).
-intros; rewrite <- H; apply PPermut_LF_get_2.
+Lemma PPermut_Hyb_tactic_simpl : forall l1 l2 l3 l4,
+  PPermut_Hyb (l1 ++ l3) l4 ->
+  PPermut_Hyb (l1 ++ (l2 ++ l3)) (l2 ++ l4).
+intros; rewrite <- H; apply PPermut_Hyb_get_2.
 Qed.
 
-Lemma PPermut_LF_tactic_trans : forall l1 l2 l3,
-  PPermut_LF l3 l2 -> PPermut_LF l1 l3 -> PPermut_LF l1 l2.
+Lemma PPermut_Hyb_tactic_trans : forall l1 l2 l3,
+  PPermut_Hyb l3 l2 -> PPermut_Hyb l1 l3 -> PPermut_Hyb l1 l2.
 intros; eauto with ppermut_rew.
 Qed.
 
 Hint Rewrite app_assoc app_nil_l app_nil_r : ppermut_rew.
 
-Ltac PPermut_LF_lemma_get n :=
+Ltac PPermut_Hyb_lemma_get n :=
   match nat_from_number n with
-  | 1 => constr:(PPermut_LF_get_1)
-  | 2 => constr:(PPermut_LF_get_2)
-  | 3 => constr:(PPermut_LF_get_3)
-  | 4 => constr:(PPermut_LF_get_4)
-  | 5 => constr:(PPermut_LF_get_5)
+  | 1 => constr:(PPermut_Hyb_get_1)
+  | 2 => constr:(PPermut_Hyb_get_2)
+  | 3 => constr:(PPermut_Hyb_get_3)
+  | 4 => constr:(PPermut_Hyb_get_4)
+  | 5 => constr:(PPermut_Hyb_get_5)
   end.
 
-Ltac PPermut_LF_isolate_cons :=
+Ltac PPermut_Hyb_isolate_cons :=
   do 20 try (* todo : repeat *)
     match goal with |- context [?x::?l] =>
       match l with
@@ -186,14 +186,14 @@ Ltac PPermut_LF_isolate_cons :=
       end
     end.
 
-Ltac PPermut_LF_simpl_prepare :=
+Ltac PPermut_Hyb_simpl_prepare :=
    autorewrite with ppermut_rew;
-   PPermut_LF_isolate_cons;
+   PPermut_Hyb_isolate_cons;
    autorewrite with ppermut_rew;
-   apply PPermut_LF_tactic_setup;
+   apply PPermut_Hyb_tactic_setup;
    repeat rewrite app_assoc.
 
-Ltac PPermut_LF_index_of l lcontainer :=
+Ltac PPermut_Hyb_index_of l lcontainer :=
   match constr:(lcontainer) with
   | l ++ _ => constr:(1)
   | _ ++ l ++ _ => constr:(2)
@@ -204,32 +204,33 @@ Ltac PPermut_LF_index_of l lcontainer :=
   | _ => constr:(0) (* not found *)
   end.
 
-Ltac PPermut_LF_simpl_once :=
+Ltac PPermut_Hyb_simpl_once :=
   match goal with
-  | |- PPermut_LF (_ ++ nil) _ => fail 1
-  | |- PPermut_LF (_ ++ (?l ++ _)) ?l' =>
-     match PPermut_LF_index_of l l' with
-     | 0 => apply PPermut_LF_tactic_keep
-     | ?n => let F := PPermut_LF_lemma_get n in
-            eapply PPermut_LF_tactic_trans;
+  | |- PPermut_Hyb (_ ++ nil) _ => fail 1
+  | |- PPermut_Hyb (_ ++ (?l ++ _)) ?l' =>
+     match PPermut_Hyb_index_of l l' with
+     | 0 => apply PPermut_Hyb_tactic_keep
+     | ?n => let F := PPermut_Hyb_lemma_get n in
+            eapply PPermut_Hyb_tactic_trans;
             [ apply F
-            | apply PPermut_LF_tactic_simpl ]
+            | apply PPermut_Hyb_tactic_simpl ]
      end
   end.
 
-Ltac PPermut_LF_simpl :=
-  PPermut_LF_simpl_prepare;
-  repeat PPermut_LF_simpl_once;
+Ltac PPermut_Hyb_simpl :=
+  PPermut_Hyb_simpl_prepare;
+  repeat PPermut_Hyb_simpl_once;
   autorewrite with ppermut_rew;
-  try apply PPermut_LF_reflexive;
+  try apply PPermut_Hyb_reflexive;
   auto.
 
 
 (*** Other lemmas ***)
 (* Note:
-   Some are covered by PPermut_LF_simpl tactic, but we want to use them in auto! *)
+   Some are covered by PPermut_Hyb_simpl tactic, but we want to use them
+   in auto! *)
 
-Lemma PPermut_LF_Mem:
+Lemma PPermut_Hyb_Mem:
 forall G G' w X,
   G ~=~ G' ->
   Mem (w, X) G ->
@@ -238,7 +239,7 @@ intros; generalize dependent X; induction H; intros.
 rewrite Mem_nil_eq in H0; contradiction.
 rewrite Mem_cons_eq in H1; destruct H1.
 inversion H1; subst; exists Gamma'; split; [ symmetry | apply Mem_here]; auto.
-apply IHPPermut_LF in H1; destruct H1 as (Gamma''); exists Gamma'';
+apply IHPPermut_Hyb in H1; destruct H1 as (Gamma''); exists Gamma'';
 destruct H1; split; auto; rewrite Mem_cons_eq; right; auto.
 repeat rewrite Mem_cons_eq in H1; destruct H1.
 inversion H1; subst; exists Gamma1; split; [ symmetry | rewrite Mem_cons_eq];
@@ -247,31 +248,31 @@ destruct H1.
 inversion H1; subst; exists Gamma1'; split; [ symmetry | rewrite Mem_cons_eq];
 auto.
 exists X; split; auto; repeat rewrite Mem_cons_eq; right; right; auto.
-apply IHPPermut_LF1 in H1; destruct H1 as (X'); destruct H1.
-apply IHPPermut_LF2 in H2; destruct H2 as (X''); destruct H2;
+apply IHPPermut_Hyb1 in H1; destruct H1 as (X'); destruct H1.
+apply IHPPermut_Hyb2 in H2; destruct H2 as (X''); destruct H2;
 exists X''; split; auto; transitivity X'; auto.
 Qed.
 
-Lemma PPermut_LF_nil_impl:
+Lemma PPermut_Hyb_nil_impl:
 forall L,
   nil ~=~ L -> L = nil.
-intros; remember (@nil Context_LF) as L' in H;
+intros; remember (@nil ctx_Hyb) as L' in H;
 induction H; intros;
 discriminate || auto.
 Qed.
 
-Lemma PPermut_LF_nil_contr:
+Lemma PPermut_Hyb_nil_contr:
 forall L a,
-  ~ (PPermut_LF nil (a::L)).
+  ~ (PPermut_Hyb nil (a::L)).
 induction L; intros; intro;
-apply PPermut_LF_nil_impl in H; discriminate.
+apply PPermut_Hyb_nil_impl in H; discriminate.
 Qed.
 
-Hint Resolve PPermut_LF_nil_impl PPermut_LF_nil_contr.
+Hint Resolve PPermut_Hyb_nil_impl PPermut_Hyb_nil_contr.
 
 (* Based on Sorting/Permutation/Permutation_ind_bis *)
-Theorem PPermut_LF_ind_bis :
- forall P : list Context_LF -> list Context_LF -> Prop,
+Theorem PPermut_Hyb_ind_bis :
+ forall P : list ctx_Hyb -> list ctx_Hyb -> Prop,
    P nil nil ->
    (forall w x y l l', l ~=~ l' -> P l l' ->
      x *=* y -> P ((w,x) :: l) ((w,y) :: l')) ->
@@ -289,7 +290,7 @@ Proof.
   eauto.
 Qed.
 
-Lemma PPermut_LF_app_rev:
+Lemma PPermut_Hyb_app_rev:
 forall G G' H H' w a a',
   a *=* a' ->
   G & (w, a) ++ G' ~=~ H & (w, a') ++ H' ->
@@ -300,7 +301,7 @@ Proof.
          l=l1 & (w, a) ++ l2 -> l'=l3 & (w, a') ++l4 -> (l1++l2) ~=~ (l3++l4)).
   cut (forall l l', l ~=~ l' -> P l l').
   intros; apply (H _ _ H2 w a a'); auto.
-  intros; apply (PPermut_LF_ind_bis P); unfold P; clear P;
+  intros; apply (PPermut_Hyb_ind_bis P); unfold P; clear P;
     try clear H l l'; simpl; auto.
   (* nil *)
   intros; destruct l1; simpl in *; discriminate.
@@ -308,9 +309,9 @@ Proof.
   intros w x y l l' H IH; intros.
   destruct l1; destruct l3; rew_app in *;
   inversion H2; inversion H3; subst; auto.
-    rewrite H; PPermut_LF_simpl; constructor; [transitivity a |] ; auto;
+    rewrite H; PPermut_Hyb_simpl; constructor; [transitivity a |] ; auto;
       symmetry; auto.
-    rewrite <- H; PPermut_LF_simpl; constructor; auto; transitivity a';
+    rewrite <- H; PPermut_Hyb_simpl; constructor; auto; transitivity a';
       [ | symmetry]; auto.
   constructor; auto.
   apply (IH w0 a a' l1 l2 l3 l4); rew_app; auto.
@@ -318,52 +319,52 @@ Proof.
   intros w w' x x' y y' l l' Hp IH; intros.
   destruct l1; destruct l2; rew_app in *; subst;
   inversion H2; subst; auto; try rewrite Hp; rew_app;
-  PPermut_LF_simpl; destruct l3; destruct l4; rew_app in *; subst;
+  PPermut_Hyb_simpl; destruct l3; destruct l4; rew_app in *; subst;
   inversion H3; subst; auto.
     constructor; auto; transitivity a'; auto; transitivity a; auto;
     symmetry; auto.
     constructor; auto; destruct l3; rew_app in *; inversion H6; subst; auto;
-      PPermut_LF_simpl; constructor; auto; transitivity a; auto; symmetry; auto.
+      PPermut_Hyb_simpl; constructor; auto; transitivity a; auto; symmetry; auto.
     constructor; auto; destruct l3; rew_app in *; inversion H6; subst; auto;
-      PPermut_LF_simpl; constructor; auto; transitivity a; auto; symmetry; auto.
+      PPermut_Hyb_simpl; constructor; auto; transitivity a; auto; symmetry; auto.
     constructor; auto; destruct l1; rew_app in *; inversion H6; subst; auto;
-      PPermut_LF_simpl; rewrite <- Hp; PPermut_LF_simpl; constructor; auto;
+      PPermut_Hyb_simpl; rewrite <- Hp; PPermut_Hyb_simpl; constructor; auto;
       transitivity a'; auto; symmetry; auto.
   destruct l1; destruct l3; rew_app in *; inversion H6; inversion H7; subst;
     auto.
       constructor; auto; transitivity a'; auto; transitivity a; auto;
         symmetry; auto.
-       apply PPermut_LF_nil_impl in Hp; destruct l3; rew_app in *; discriminate.
-       symmetry in Hp; apply PPermut_LF_nil_impl in Hp; destruct l1; rew_app in *;
-         discriminate.
+       apply PPermut_Hyb_nil_impl in Hp; destruct l3; rew_app in *; discriminate.
+       symmetry in Hp; apply PPermut_Hyb_nil_impl in Hp; destruct l1;
+         rew_app in *; discriminate.
        transitivity ((w', y') :: (w, x') :: l1).
          constructor; [ | constructor]; auto.
-         PPermut_LF_simpl.
+         PPermut_Hyb_simpl.
        replace l1 with (l1 ++ nil) by (rew_app; auto);
        replace l3 with (l3 ++ nil) by (rew_app; auto);
        apply IH with (w:=w0) (a0:=a) (a'0:=a'); auto;
          rew_app; auto.
   destruct l1; destruct l3; rew_app in *; inversion H6; inversion H7; subst;
     auto.
-       apply PPermut_LF_nil_impl in Hp; discriminate.
-       apply PPermut_LF_nil_impl in Hp; destruct l3; rew_app in *; discriminate.
-       rewrite <- Hp; PPermut_LF_simpl; transitivity ((w,x)::(w0,y)::nil);
-         PPermut_LF_simpl; constructor; auto; constructor; auto; transitivity a';
-         auto; symmetry; auto.
-       transitivity ((w',y')::(w,x')::l1); auto; PPermut_LF_simpl; rew_app;
+       apply PPermut_Hyb_nil_impl in Hp; discriminate.
+       apply PPermut_Hyb_nil_impl in Hp; destruct l3; rew_app in *; discriminate.
+       rewrite <- Hp; PPermut_Hyb_simpl; transitivity ((w,x)::(w0,y)::nil);
+         PPermut_Hyb_simpl; constructor; auto; constructor; auto;
+         transitivity a'; auto; symmetry; auto.
+       transitivity ((w',y')::(w,x')::l1); auto; PPermut_Hyb_simpl; rew_app;
        replace l1 with (l1 ++ nil) by (rew_app; auto);
        apply IH with (w:=w0) (a0:=a) (a'0:=a'); auto;
          rew_app; auto.
   constructor; auto; rewrite <- Hp; symmetry; destruct l1; rew_app in *;
-    inversion H6; subst; auto; PPermut_LF_simpl; constructor; auto;
+    inversion H6; subst; auto; PPermut_Hyb_simpl; constructor; auto;
     transitivity a'; auto; symmetry; auto.
   destruct l3; rew_app in *; inversion H7; subst.
-    symmetry in Hp; apply PPermut_LF_nil_impl in Hp; subst; inversion H6; subst;
+    symmetry in Hp; apply PPermut_Hyb_nil_impl in Hp; subst; inversion H6; subst;
       destruct l1; rew_app in *; inversion H6; subst; destruct l1; rew_app in *;
       discriminate.
-    transitivity ((w', y') ::l1 ++ p0 :: l2); PPermut_LF_simpl; rew_app.
+    transitivity ((w', y') ::l1 ++ p0 :: l2); PPermut_Hyb_simpl; rew_app.
     destruct l1; rew_app in *; inversion H6; subst.
-      rewrite Hp; PPermut_LF_simpl; constructor; auto; transitivity a; auto;
+      rewrite Hp; PPermut_Hyb_simpl; constructor; auto; transitivity a; auto;
       symmetry; auto.
       constructor; auto; replace l3 with (l3 ++ nil) by (rew_app; auto);
       apply IH with (w:=w0) (a0:=a) (a'0:=a'); auto; rew_app; auto.
@@ -373,21 +374,21 @@ Proof.
     symmetry; auto.
     transitivity ((w', y'):: p0 :: l2).
       constructor; auto.
-      PPermut_LF_simpl. clear H6 H7. rew_app; rewrite Hp; PPermut_LF_simpl;
+      PPermut_Hyb_simpl. clear H6 H7. rew_app; rewrite Hp; PPermut_Hyb_simpl;
       constructor; auto; transitivity a; auto; symmetry; auto.
     transitivity ((w, x)::p1::l4).
-      PPermut_LF_simpl; rew_app; rewrite <- Hp; PPermut_LF_simpl; constructor;
+      PPermut_Hyb_simpl; rew_app; rewrite <- Hp; PPermut_Hyb_simpl; constructor;
         auto; transitivity a'; auto; symmetry; auto.
       constructor; auto.
     transitivity ((w', y') :: (w, x') :: l1 ++ p0 :: l2).
       constructor; auto; constructor; auto.
-      PPermut_LF_simpl. clear H7 H6. rew_app.
+      PPermut_Hyb_simpl. clear H7 H6. rew_app.
     apply IH with (w:=w0) (a0:=a) (a'0:=a'); rew_app; auto.
   (* trans *)
-  intros. destruct (PPermut_LF_Mem l l' w a) as (a'', (H6a, H6b)); auto.
+  intros. destruct (PPermut_Hyb_Mem l l' w a) as (a'', (H6a, H6b)); auto.
     subst; rewrite Mem_app_or_eq; left; rewrite Mem_app_or_eq; right;
       apply Mem_here.
-  destruct (Mem_split Context_LF l' (w, a'')) as (l'1, (l'2, H6)); auto.
+  destruct (Mem_split ctx_Hyb l' (w, a'')) as (l'1, (l'2, H6)); auto.
   transitivity (l'1 ++ l'2).
     apply H0 with (w:=w) (a:=a) (a':=a''); [ symmetry | | ]; auto.
     apply H2 with (w:=w) (a:=a'') (a':=a').
@@ -396,35 +397,35 @@ Proof.
       auto.
 Qed.
 
-Lemma PPermut_LF_last_rev_simpl:
+Lemma PPermut_Hyb_last_rev_simpl:
 forall G G' a,
   G & a ~=~ G' & a ->
   G ~=~ G'.
 intros. replace G with (G ++ nil);
 replace G' with (G'++nil).
-destruct a; eapply PPermut_LF_app_rev; rew_app; eauto.
+destruct a; eapply PPermut_Hyb_app_rev; rew_app; eauto.
 rew_app; auto.
 rew_app; auto.
 rew_app; auto.
 Qed.
 
-Lemma PPermut_LF_last_rev:
+Lemma PPermut_Hyb_last_rev:
 forall G G' w Gamma Gamma',
   Gamma *=* Gamma' ->
   G & (w, Gamma) ~=~ G' & (w, Gamma') ->
   G ~=~ G'.
 intros;
 assert (G & (w, Gamma) ~=~ G' & (w, Gamma)) by eauto with ppermut_rew;
-apply PPermut_LF_last_rev_simpl with (a:=(w, Gamma)); auto.
+apply PPermut_Hyb_last_rev_simpl with (a:=(w, Gamma)); auto.
 Qed.
 
-Lemma PPermut_LF_split_head:
+Lemma PPermut_Hyb_split_head:
 forall G G' w Gamma,
   (w, Gamma) :: G ~=~ G' ->
   exists Gamma' hd tl,
     Gamma *=* Gamma' /\ G' = hd & (w, Gamma') ++ tl.
 intros.
-apply PPermut_LF_Mem with (w:=w) (X:=Gamma) in H.
+apply PPermut_Hyb_Mem with (w:=w) (X:=Gamma) in H.
 destruct H as (Gamma'); destruct H.
 exists Gamma'.
 assert (exists hd, exists tl, G' = hd & (w, Gamma') ++ tl) by
@@ -434,7 +435,7 @@ exists hd; exists tl; split; [symmetry | ]; auto.
 apply Mem_here.
 Qed.
 
-Lemma PPermut_LF_split_neq:
+Lemma PPermut_Hyb_split_neq:
 forall G G' w w' Gamma Gamma',
   G & (w, Gamma) ~=~ G' & (w', Gamma') ->
   ~Gamma *=* Gamma' \/ w <> w' ->
@@ -443,11 +444,12 @@ forall G G' w w' Gamma Gamma',
     G = GH & (w', Gamma0) ++ GT.
 intros.
 assert ((w, Gamma) ::G  ~=~ (G' & (w', Gamma'))) by
-  (transitivity (G & (w,Gamma)); auto; PPermut_LF_simpl).
+  (transitivity (G & (w,Gamma)); auto; PPermut_Hyb_simpl).
 assert ((w, Gamma) :: G ~=~ (w', Gamma') :: G') by
-  (transitivity (G' & (w', Gamma')); auto; PPermut_LF_simpl).
+  (transitivity (G' & (w', Gamma')); auto; PPermut_Hyb_simpl).
 symmetry in H2;
-apply PPermut_LF_split_head in H2; destruct H2 as (Gamma'',(GH, (GT, (Ha, Hb)))).
+apply PPermut_Hyb_split_head in H2;
+destruct H2 as (Gamma'',(GH, (GT, (Ha, Hb)))).
 destruct GH; rew_app in *.
 inversion Hb; subst; destruct H0; elim H0; symmetry; auto.
 destruct p; inversion Hb; subst.
@@ -455,100 +457,100 @@ exists Gamma''; exists GH; exists GT; split;
 [symmetry | rew_app]; auto.
 Qed.
 
-Lemma PPermut_LF_swap2:
+Lemma PPermut_Hyb_swap2:
 forall C C' G,
   C :: G & C' ~=~ G & C & C'.
-intros; PPermut_LF_simpl.
+intros; PPermut_Hyb_simpl.
 Qed.
-Hint Resolve PPermut_LF_swap2.
+Hint Resolve PPermut_Hyb_swap2.
 
-Lemma PPermut_LF_middle_last:
+Lemma PPermut_Hyb_middle_last:
 forall G G' C,
   G ++ G' & C ~=~ G ++ C :: G'.
-intros; PPermut_LF_simpl.
+intros; PPermut_Hyb_simpl.
 Qed.
-Hint Resolve PPermut_LF_middle_last.
+Hint Resolve PPermut_Hyb_middle_last.
 
-Lemma PPermut_LF_specialized1:
+Lemma PPermut_Hyb_specialized1:
 forall G G' C C',
   G ++ C :: G' & C' ~=~ G ++ G' ++ C' :: C :: nil.
-intros; PPermut_LF_simpl.
+intros; PPermut_Hyb_simpl.
 Qed.
 
-Lemma PPermut_LF_specialized2:
+Lemma PPermut_Hyb_specialized2:
 forall GH GT G Gamma Gamma' Gamma'',
   GH ++ Gamma :: GT & Gamma' ~=~ G & Gamma ->
   GH ++ GT ++ Gamma'' :: Gamma' :: nil ~=~ G & Gamma''.
-intros; PPermut_LF_simpl;
-apply PPermut_LF_last_rev_simpl with (a:=Gamma);
-rewrite <- H; PPermut_LF_simpl.
+intros; PPermut_Hyb_simpl;
+apply PPermut_Hyb_last_rev_simpl with (a:=Gamma);
+rewrite <- H; PPermut_Hyb_simpl.
 Qed.
 
-Lemma PPermut_LF_specialized3:
+Lemma PPermut_Hyb_specialized3:
 forall G G' C C',
   G ++ G' ++ C :: C' :: nil ~=~ G ++ C :: G' & C'.
-intros; PPermut_LF_simpl.
+intros; PPermut_Hyb_simpl.
 Qed.
 
-Lemma PPermut_LF_specialized4:
+Lemma PPermut_Hyb_specialized4:
 forall G GH GT Gamma Gamma0 Gamma'0,
   GH ++ Gamma :: GT & Gamma'0 ~=~ G & Gamma ->
   G ++ Gamma0 :: Gamma :: nil ~=~ GH ++ GT ++ Gamma0 :: Gamma'0 :: Gamma :: nil.
-intros; PPermut_LF_simpl;
-apply PPermut_LF_last_rev_simpl with (a:=Gamma); rewrite <- H;
-PPermut_LF_simpl.
+intros; PPermut_Hyb_simpl;
+apply PPermut_Hyb_last_rev_simpl with (a:=Gamma); rewrite <- H;
+PPermut_Hyb_simpl.
 Qed.
 
-Lemma PPermut_LF_specialized5:
+Lemma PPermut_Hyb_specialized5:
 forall G G' C C' C'',
   G ++ C :: G' ++ C' :: C'' :: nil ~=~ (G ++ G' ++ C' :: C'' :: nil) & C.
-intros; PPermut_LF_simpl.
+intros; PPermut_Hyb_simpl.
 Qed.
 
-Lemma PPermut_LF_specialized6:
+Lemma PPermut_Hyb_specialized6:
 forall GH GT C0 C'' C'0,
   GH ++ GT ++ C'0 :: C'' :: C0 :: nil ~=~ GH ++ GT ++ C0 :: C'0 :: C'' :: nil.
-intros; PPermut_LF_simpl.
+intros; PPermut_Hyb_simpl.
 Qed.
 
-Lemma PPermut_LF_swap_inner:
+Lemma PPermut_Hyb_swap_inner:
 forall G G' C C',
   C :: G ++ C' :: G' ~=~ C' :: G ++ G' & C.
-intros; PPermut_LF_simpl.
+intros; PPermut_Hyb_simpl.
 Qed.
 
-Lemma PPermut_LF_swap_inner2:
+Lemma PPermut_Hyb_swap_inner2:
 forall G G' C C',
   C :: G ++ G' & C' ~=~ C' :: G ++ G' & C.
-intros; PPermut_LF_simpl.
+intros; PPermut_Hyb_simpl.
 Qed.
 
-Lemma PPermut_LF_swap3:
+Lemma PPermut_Hyb_swap3:
 forall C C' G,
   C :: G & C' ~=~ C' :: G & C.
-intros; PPermut_LF_simpl.
+intros; PPermut_Hyb_simpl.
 Qed.
 
-Lemma PPermut_LF_swap4:
+Lemma PPermut_Hyb_swap4:
 forall C G' G,
   G ++ G' & C ~=~ G & C ++ G'.
-intros; PPermut_LF_simpl.
+intros; PPermut_Hyb_simpl.
 Qed.
 
-Hint Resolve PPermut_LF_swap_inner.
-Hint Resolve PPermut_LF_swap_inner2.
-Hint Resolve PPermut_LF_swap3 PPermut_LF_swap4.
+Hint Resolve PPermut_Hyb_swap_inner.
+Hint Resolve PPermut_Hyb_swap_inner2.
+Hint Resolve PPermut_Hyb_swap3 PPermut_Hyb_swap4.
 
-Hint Resolve PPermut_LF_specialized2 : ppermut_rew.
-Hint Resolve PPermut_LF_specialized1
-             PPermut_LF_specialized3 PPermut_LF_specialized4
-             PPermut_LF_specialized5 PPermut_LF_specialized6.
+Hint Resolve PPermut_Hyb_specialized2 : ppermut_rew.
+Hint Resolve PPermut_Hyb_specialized1
+             PPermut_Hyb_specialized3 PPermut_Hyb_specialized4
+             PPermut_Hyb_specialized5 PPermut_Hyb_specialized6.
 
-Lemma permut_PPermut_LF:
+Lemma permut_PPermut_Hyb:
 forall G G', G *=* G' -> G ~=~ G'.
 intros. induction H; auto.
 transitivity y; auto.
-inversion H. PPermut_LF_simpl.
+inversion H. PPermut_Hyb_simpl.
 Qed.
 
 Close Scope permut_scope.
